- Change concrete machine to use Z tags instead of labels throughout. - Change Push instruction to take a bare Z rather than an atom; many consequent simplifications since instructions no longer depend on lattice. - Add BOT as a symbolic label expression, with associated genBot code and proof of correctness.  (This is needed so that rule for Push can return bottom.) - Rename glue functions and move them to FaultHandler.v

ifc-machine/pico/Altogether.v
@@ -21,6 +21,8 @@ Require Import AbstractObsEquiv NIAbstractMachine.
 Require Import Concrete ConcreteMachine CodeGen.
 Require Import FaultRoutine.
 
+Require Import Refinement.
+
 Set Implicit Arguments.
 Local Open Scope Z_scope. 
 (** This file summarizes the results we already have and the one we aim at *)
@@ -33,7 +35,7 @@ Context {L: Type} {Latt: JoinSemiLattice L}.
 (** Initial state of the abstract machine *)
 Variable mty : list (@Atom L) -> Prop.
 
-Inductive initial_astate (P: list (@Instr L)) : @AS L -> Prop :=
+Inductive initial_astate (P: list Instr) : @AS L -> Prop :=
 | init_as: forall m, 
              mty m ->
              initial_astate P (AState m P nil (0,bot)).
@@ -41,7 +43,7 @@ Inductive initial_astate (P: list (@Instr L)) : @AS L -> Prop :=
 (** * Non-interference property on the abstract Machine *)
 
 (** Defining observation, execution traces, and indistingability relation *)
-Let low_equiv_prog := fun o => low_equiv_list (low_equiv_instr o).
+Let low_equiv_prog := fun (o:L) => low_equiv_list (low_equiv_instr o).
 Let observe_astate : @AS L -> @AS L := (fun x => x).
 Let aexec_with_trace := sys_trace step_rules success observe_astate.
 Let indistinguishable := lockstep_indist low_pc success low_equiv_full_state.
@@ -62,21 +64,26 @@ Context {CLatt: ConcreteLattice L}.
 
 (** The fault handler code *)
 Definition faultHandler := FaultRoutine.faultHandler (fun opcode => existT _ (labelCount opcode) (fetch_rule opcode)).
-Variable mtyCache : list (@Atom L).
+Variable mtyCache : list (@Atom Z).
 
 (** Initial state of the concrete machine *)
-Inductive initial_cstate (P: list (@Instr L)) : @CS L -> Prop :=
-| init_cs : forall m, initial_cstate P (CState mtyCache m faultHandler P nil (0,bot) false).
+Inductive initial_cstate (P: list Instr) : CS -> Prop :=
+| init_cs : forall m, initial_cstate P (CState mtyCache m faultHandler P nil (0,labToZ bot) false).
 
+(* Now defined in Refinement ...
 (** Aux functions yet to be defined *)
-Variable c_to_a_stack : list (@CStkElmt L) -> list (@StkElmt L). 
+Variable c_to_a_stack : list CStkElmt -> list (@StkElmt L). 
+
+Variable c_to_a_mem : list (@Atom L) -> list (@Atom Z).
 
 (** Observing a concete cache is just projecting it a the abstract level *)
-Let observe_cstate (cs: @CS L) : @AS L := 
+Let observe_cstate (cs: CS) : @AS L := 
   match cs with 
-    | CState c m fh i s pc p => AState m i (c_to_a_stack s) pc
+    | CState c m fh i s pc p => AState (c_to_a_mem m) i (c_to_a_stack s) (ZToLab pc)
   end.
   
+*)
+
 Let cexec_with_trace := sys_trace cstep c_success observe_cstate.
 
 Theorem NI_concrete_machine: forall o P P' s s' T T', 
