ifc-machine/pico/tmu/cmach/WfCLattices.v
@@ -13,22 +13,26 @@ Require Import CodeSpecs.
 (* Lattice-dependent parameters *)
 Class WfConcreteLattice (T: Type) (L : JoinSemiLattice T) (CL: ConcreteLattice T) :=
 { ZToLab_labToZ_id: forall l, l = ZToLab (labToZ l)
+; genBot_spec: forall m0 s0,
+   HT genBot
+       (fun m s => m = m0 /\ s = s0)
+       (fun m s => m = m0 /\ s = CData (labToZ bot, handlerTag) :: s0)
 ; genJoin_spec: forall l l' m0 s0,
    HT  genJoin
        (fun m s => m = m0 /\
-                   s = CData (labToZ l, handlerLabel) ::
-                       CData (labToZ l', handlerLabel) :: s0)
+                   s = CData (labToZ l, handlerTag) ::
+                       CData (labToZ l', handlerTag) :: s0)
        (fun m s => m = m0 /\
-                   s = CData (labToZ (join l l'), handlerLabel) :: s0)
+                   s = CData (labToZ (join l l'), handlerTag) :: s0)
   (* NC: we could discharge this by implementing [genFlows] in terms of
    [genJoin], and using the fact that [flows l l' = true <-> join l l' = l']. *)
 ; genFlows_spec: forall l l' m0 s0,
    HT  genFlows
        (fun m s => m = m0 /\
-                   s = CData (labToZ l, handlerLabel) ::
-                       CData (labToZ l', handlerLabel) :: s0)
+                   s = CData (labToZ l, handlerTag) ::
+                       CData (labToZ l', handlerTag) :: s0)
        (fun m s => m = m0 /\
-                   s = CData (boolToZ (flows l l'), handlerLabel) :: s0)
+                   s = CData (boolToZ (flows l l'), handlerTag) :: s0)
 }.
 
 Lemma labToZ_inj: forall {L J C} {W: WfConcreteLattice L J C} (l1 l2: L),
@@ -49,13 +53,23 @@ Proof.
   destruct l; auto.
 Qed.
 
+Lemma genBot_spec' : forall m0 s0,
+   HT genBot
+       (fun m s => m = m0 /\ s = s0)
+       (fun m s => m = m0 /\ s = CData (labToZ bot, handlerTag) :: s0).
+Proof.
+   intros.
+   unfold genBot, TMUHL. 
+   eapply genFalse_spec; simpl; eauto.
+Qed.
+
 Lemma genJoin_spec' : forall l l' m0 s0,
    HT  genJoin
        (fun m s => m = m0 /\
-                   s = CData (labToZ l, handlerLabel) ::
-                       CData (labToZ l', handlerLabel) :: s0)
+                   s = CData (labToZ l, handlerTag) ::
+                       CData (labToZ l', handlerTag) :: s0)
        (fun m s => m = m0 /\
-                   s = CData (labToZ (join l l'), handlerLabel) :: s0).
+                   s = CData (labToZ (join l l'), handlerTag) :: s0).
 Proof.
   intros.
   unfold genJoin, TMUHL. 
@@ -67,10 +81,10 @@ Qed.
 Lemma genFlows_spec': forall l l' m0 s0,
    HT  genFlows
        (fun m s => m = m0 /\
-                   s = CData (labToZ l, handlerLabel) ::
-                       CData (labToZ l', handlerLabel) :: s0)
+                   s = CData (labToZ l, handlerTag) ::
+                       CData (labToZ l', handlerTag) :: s0)
        (fun m s => m = m0 /\
-                   s = CData (boolToZ (flows l l'), handlerLabel) :: s0).
+                   s = CData (boolToZ (flows l l'), handlerTag) :: s0).
 Proof.
   intros.
   unfold genFlows, TMUHL.
@@ -81,6 +95,7 @@ Qed.
 
 Instance TMUHLwf : WfConcreteLattice Lab HL TMUHL :=
 { ZToLab_labToZ_id := ZToLab_labToZ_id'
+; genBot_spec := genBot_spec'
 ; genJoin_spec := genJoin_spec'
 ; genFlows_spec := genFlows_spec'
 }.
@@ -109,10 +124,10 @@ Module HL : TMULattice.
   Definition T := Lab. 
   Definition Latt := HL. 
 
-  Definition handlerLabel := H. 
+  Definition handlerTag := H. 
 
   Definition pop := (@BranchNZ T) 1. 
-  Definition push v := Push (v,handlerLabel).
+  Definition push v := Push (v,handlerTag).
   Definition branch ofs := 
   [push 1;
    BranchNZ (if ofs >=? 0 then ofs else ofs - 1 )]. 
